<?xml version="1.0" encoding="UTF-8" ?>
<!-- **********************************************************************-->
<!-- Copyright 2019                                                        -->
<!-- UNL Department of Mathematics                                         -->
<!-- Based upon the work of                                                -->
<!-- Matthew Boelkins                                                      -->
<!-- Copyright 2012-2018                                                   -->
<!--                                                                       -->
<!-- This file is part of Coordinated Calculus.                            -->
<!-- This file is based on Active Calculus.                                -->
<!--                                                                       -->
<!-- Permission is granted to copy, distribute and/or modify this document -->
<!-- under the terms of the Creative Commons BY-SA license.  The work      -->
<!-- may be used for free by any party so long as attribution is given to  -->
<!-- the author(s), the work and its derivatives are used in the spirit of -->
<!-- "share and share alike".  All trademarks are the registered marks of  -->
<!-- their respective owners.                                              -->
<!-- **********************************************************************-->
<section xmlns:xi="http://www.w3.org/2001/XInclude" xml:id="sec-2-4-2-tan-line" permid="TnL">
  <title>The Tangent Line</title>
  <objectives permid="ADl">
    <ul permid="AjD">
      <li permid="EmL">
        <p permid="CAl">
          What is a tangent line? 
        </p>
      </li>

      <li permid="CaK">
        <p permid="STk">
         How can we sketch a tangent line? 
        </p>
      </li>

      <li permid="xyx">
        <p permid="TgB">
          How do we find an equation for the tangent line? 
  
        </p>
      </li>
    </ul>
  </objectives>


  <introduction permid="MHv">
    <p permid="oOF">
Recall that a line can be written as <m> y = m(x- x_0) + y_0</m>, where <m> m </m> is the slope of the line and 
<m> (x_0, y_0) </m> is a point on the line. Using this information and our new derivative rules, we are in a position to 
quickly find the equation for the line which intersects a curve at a particular point and has the same slope, which we call
the <em> tangent line </em>. Specifically, we have the following definition. 
    </p>

 <p xml:id="Tandef" permid="Tandef">
 <idx><h>tangent line</h><h>equation</h></idx>
 <assemblage><title>The Tangent Line</title>
 <p>Given a differentiable function <m>f</m> and a point <m>(x_0,y_0)</m> the equation for the <term>tangent line to the function <m>f</m> at <m>(x_0,y_0)</m></term> is given by
 <me>y=f'(x_0)(x-x_0)+y_0.</me></p>
 </assemblage>
 </p>
 
<p>We will look more at tangent lines in future sections but the basic ideas appear here.  Specifically, if we know data about a function at a specific point such as it's value at that point and rate of change at that point then we can estimate its value at a future point.</p>

  </introduction>

  <subsection permid="yDQ">
    <title>Sketching the Tangent Line</title>
    <p permid="BcX">
     If the tangent line at <m>x = a</m> exists,
      the graph of <m>f</m> looks like a straight line when viewed up close at <m>(a,f(a))</m>.
      In <xref ref="F-2-4">Figure</xref> below,
      we zoom in on <m>f(x)</m> and its tangent line at <m>(a,f(a))</m>. Note how the tangent line sits relative to the curve <m>y = f(x)</m> at
      <m>(a,f(a))</m>, and how closely it resembles the curve near <m>x = a</m>.
    </p>
        <figure xml:id="F-2-4" permid="cOR">
      <caption>Zooming in on <m> f(x) </m> and its tangent line at <m> x = a</m>.</caption>
      <image width="100%" source="images/1-8-TanLines.gif"/>
    </figure>

    <p>
    With this information, we may informally <em>sketch</em> a tangent line by estimating the rate of change at a point <m> x = a </m>
and following a straight line. 
    </p> 
    <example>
    <statement>

    <p>
    Below in <xref ref="FF2">Figure</xref> is the graph of a function, <m> g(x) </m>. We can sketch the tangent line at several different 
    points.
    </p>
      <figure xml:id="FF2" permid="ElI">
        <caption> Graph of <m> g(x) </m>. </caption>
        <image width="80%" source="images/2-4-plot.jpg"/>
      </figure>
    <p>Notice that at the point <m> x = -2</m>, the slope of the tangent line is positive, and at the point <m> x = 2 </m>, the slope of the tangent line is negative.</p>
    <sidebyside widths="45% 45%" valign="middle">
      <figure xml:id="F-2-5" permid="JfT">
        <caption> Tangent line, dashed, at <m> x = -2 </m>.</caption>
        <image width="80%" source="images/2-4-tan1.jpg"/>
      </figure>
      <figure xml:id="F-2-6" permid="AnD">
        <caption> Tangent line, dashed, at <m> x = 2 </m>.</caption>
        <image width="80%" source="images/2-4-tan2.jpg"/>
      </figure>
    </sidebyside>
    <p> At roughly <m> x = 3.7 </m>, the slope of the tangent line is zero. </p>
    <sidebyside width="45%" valign="middle">
      <figure xml:id="F-2-7" permid="D0v">
        <caption> Tangent line, dashed, at <m> x \approx 3.7 </m>.</caption>
        <image width="80%" source="images/2-4-tan3.jpg"/>
      </figure>
    </sidebyside>  
      
    
          </statement>
    </example>

     <example>
     <statement>
     <p>
    Below is the graph of a function <m> f(x) </m>. </p>
                       <figure xml:id="F-2-8" permid="cHi">
            <caption> Graph of <m> f(x) </m>.</caption>
      <image width="80%" source="images/2_4_test.png"/>
          </figure>
    <p>Give the <m>x</m>-coordinate
    of a point where:
    <ol label="a.">

    <li>
    <p>
    The slope of the tangent line is negative.
    </p>
    </li>

        <li>
    <p>
    The slope of the tangent line is positive.
    </p>
    </li>

        <li>
    <p>
    The slope of the tangent line is zero.
    </p>
    </li>

    </ol>
    </p>
    </statement>
        <answer>
    <p>
    <ol label="a.">
      <li>
    <p>
    Any <m> x </m>-coordinate in the domain <m> (2, \infty) </m> is suitable
    </p>
    </li>

    <li>
    <p>
    Any <m> x </m>-coordinate in the domain <m> (-\infty, 2) </m> is suitable
    </p>
    </li>

      <li>
    <p>
   The only <m> x </m> coordinate with a tangent line of slope zero is <m> x = 2 </m>.
    </p>
    </li>

    </ol>
    </p>
    </answer>
    </example>
  </subsection>


<subsection permid="fTL">
    <title>Finding the Tangent Line</title>
    <p>
  When finding the tangent line for a function <m> f </m>, we need three pieces of information: 
      <ul>
      <li>
        <p>
          The value, <m> x_0 </m>, at which we are finding the tangent line.
        </p>
      </li>

      <li>
        <p>
         The value of the function at <m> x = x_0 </m>, <m> f(x_0) </m>.
        </p>
      </li>

      <li>
        <p>
        The value of the derivative at <m> x = x_0 </m>,  <m> f'(x_0) </m>.
  
        </p>
      </li>
    </ul>
    Once we have all of those pieces of information, we can plug into the given formula to find
    an equation for the tangent line. 
    </p>
    <example permid="bQt">
      <statement>
        <p permid="keM">
        Suppose <m> f(x) = -\dfrac{4}{x} </m>. To find the tangent line at <m> x = -2 </m>, we 
        find the other two pieces of necessary information:
        </p>
        <p>
        First, we find <m> f(-2) </m>: 
        <md>
<mrow>f(-2)= \mathstrut \amp \frac{-4}{-2}</mrow>
<mrow>=\mathstrut \amp 2. </mrow>
</md>
        </p>
        <p>
        Next, we find <m> f'(-2) </m>: 
        <md>
        <mrow>f'(x)= \mathstrut \amp -\left(\frac{-4}{x^2}\right)</mrow>
        <mrow>= \mathstrut \amp \frac{4}{x^2},</mrow>
        <mrow>f'(-2)= \mathstrut \amp \frac{4}{(-2)^2}</mrow>
        <mrow>= \mathstrut \amp \frac{4}{4}</mrow>
        <mrow>= \mathstrut \amp 1.</mrow>
        </md>
        </p>
        <p>
        Putting the pieces together, we have 
        <me>y = 1(x+2) +2 </me>
        as an equation for the tangent line. 
        </p>
      </statement>
    </example>

    <example>
    <statement>
    <p>
    Find an equation for the line tangent to <m>g(x)= 3\sqrt{x} - x </m>
    at <m> x = 9</m>. 
    <ol label="a.">
    <li> 
    <p>
    Compute <m> g(9) </m>; this will give you the <m> y-</m>value of the
    point on the tangent line. 
    </p>
    </li>
       <li> 
    <p>
    Compute the derivative <m>g'(x)</m>.
    </p>
    </li>
       <li> 
    <p>
    Compute <m>g'(9) </m>; this is the 
    <em> slope of the tangent </em> at <m> x = 9 </m>, the <m> x</m>-value given.
    </p>
    </li>
        <li> 
    <p>
 Put together in point slope form:
    <me>y = g'(9)(x-9) + g(9). </me>
    </p>
    </li>
    </ol>
    </p>
    </statement>
    <answer>
    <p>
    <ol label="a.">

    <li>
    <p>
    <m>g(9)= 0 </m>
    </p>
    </li>

       <li>
    <p>
    <m>g'(x)= \frac{3}{2\sqrt{x}} -1</m>
    </p>
    </li>

    <li>
    <p>
    <m>g'(9) = - \frac{1}{2}</m>
    </p>
    </li>

       <li>
    <p>
    <m>y = -\frac{1}{2}(x-9)</m>
    </p>
    </li>

    </ol>
    </p>
    </answer>
    <solution>
    <p>
    <ol label="a.">
    <li>
    <p>
     <md>
<mrow>g(9)= \mathstrut \amp 3\sqrt{9} - 9</mrow>
<mrow>=\mathstrut \amp 3(3) - 9 </mrow>
<mrow> =\mathstrut \amp 0. </mrow>
</md>
    </p>
    </li>

    <li>
    <p>
    First, we will rewrite <m> g(x) </m>:
    <me>g(x) = 3x^{1/2} - x. </me>
    Then, 
    <md>
    <mrow>g'(x) =\mathstrut \amp \frac{1}{2}\left(3x^{-1/2}\right) -1 </mrow>
    <mrow> = \mathstrut \amp \frac{3}{2\sqrt{x}}-1.</mrow>
    </md>
    </p>
    </li>

        <li>
    <p>
    Plugging in <m> x = 9 </m> into part b., 
    <md>
    <mrow>g'(9) = \mathstrut \amp \frac{3}{2\sqrt{9}} - 1 </mrow>
    <mrow> =\mathstrut \amp \frac{3}{2(3)} - 1</mrow>
    <mrow> =\mathstrut \amp \frac{1}{2} - 1</mrow>
    <mrow> =\mathstrut \amp  - \frac{1}{2}.</mrow>
    </md>
    </p>
    </li>

        <li>
    <p>
    Combining the above three parts, 
     <md>
    <mrow>y = \mathstrut \amp -\frac{1}{2}(x-9) + 0 </mrow>
    <mrow> =\mathstrut \amp -\frac{1}{2}(x-9). </mrow>
    </md>
    </p>
    </li>
    </ol>
    </p>
    </solution>
      </example>

      <example xml:id="act-2-5-6" permid="nYD">
  <statement>
    <p permid="bKl">
      Each of the following questions asks you to use derivatives to answer key questions about functions.
      Be sure to think carefully about each question and to use proper notation in your responses.
    </p>

    <p permid="HRu">
      <ol label="a." permid="Wqy">
        <li permid="CxH">
          <p permid="cPE">
            If <m>\displaystyle h(z)=\sqrt{z}+\frac1z</m>, find the slope of the tangent line to the graph of <m>y=h(z)</m> at the point where <m>z = 4</m>. 
          </p>
        </li>

        <li permid="QBm">
          <p permid="Bso">
            Find an equation for the tangent line to the curve <m>y=p(a)</m>, where
            <m>p(a) = 3a^4 - 2a^3 + 7a^2 - a + 12</m>, at the point where <m>a=-1</m>.
          </p>
        </li>

        <li permid="wIv">
          <p permid="hzx">
            What is the difference between being asked to find the <em>slope</em>
            of the tangent line (asked in (a)) and the <em>equation</em>
            of the tangent line (asked in (b))?
          </p>
        </li>
      </ol>
    </p>
  </statement>
  <answer permid="RGF">
    <p permid="PvT">
      <ol label="a." permid="Kcg">
        <li permid="TvS">
          <p permid="mjq">
            <m>\displaystyle h'(4) = \frac{3}{16}</m>.
          </p>
        </li>


        <li permid="fKk">
          <p permid="yxI">
            <m>y - 25 = -33(a+1)</m>.
          </p>
        </li>

        <li permid="LRt">
          <p permid="eER">
            The slope is a number and is only one piece of the equation, 
            which contains more information.
          </p>
        </li>
      </ol>
    </p>
  </answer>
  <solution permid="lzw">
    <p permid="joK">
      <ol label="a." permid="dUX">
        <li permid="rYC">
          <p permid="KMa">
            Note that since <m>\displaystyle h(z) = z^{\frac{1}{2}} + z^{-1}</m>,
            we have <m>\displaystyle h'(z) = \frac{1}{2}z^{-\frac{1}{2}} - z^{-2}=\frac{1}{2\sqrt{z}}-\frac{1}{z^2}</m>.
            Thus,
            <m>\displaystyle h'(4) = \frac{1}{2\sqrt4} - \frac{1}{4^2} = \frac{1}{4} - \frac{1}{16} = \frac{3}{16}</m>.
            Therefore the slope of the tangent line to the graph of <m>y=h(z)</m> at the point where <m>z = 4</m> is <m>\frac{3}{16}</m>.
          </p>
        </li>

        <li permid="EmU">
          <p permid="Xas">
            Given <m>p(a) = 3a^4 - 2a^3 + 7a^2 - a + 12</m>,
            first observe that <m>p(-1) = 3 + 2 + 7 + 1 + 12 = 25</m>,
            so the tangent line will pass through the point <m>(-1,25)</m>.
            Furthermore, since <m>p'(a) = 12a^3 - 6a^2 + 14a - 1</m>,
            we know that the slope of the tangent line is 
            <m>p'(-1) = -12 - 6 - 14 - 1 = -33</m>.
            An equation of the tangent line is therefore <m>y - 25 = -33(a+1)</m>.
            Equivalently, <m>y=-33a-8</m> is an equation of this tangent line.
          </p>
        </li>

        <li permid="kud">
          <p permid="DhB">
            Finding the slope of the tangent line only requires knowing the value of the 
            derivative at a particular input. In contrast, finding the equation of the
            tangent line additionally requires knowing the value of the original function 
            at that same input. In other words, the slope is just a number, whereas the 
            equation incorporates additional information that <mdash /> together with the slope <mdash /> is 
            sufficient to actually graph the tangent line.
          </p>
        </li>
      </ol>
    </p>
  </solution>
</example>

  </subsection>

  
  <subsection permid="qZr">
    <title>Summary</title>
    <p permid="TQv">
      <ul permid="FcW">
        <li permid="ipz">
          <p permid="LCc">
        The tangent line to the graph of <m> f(x) </m> at <m> (a, f(a)) </m> closely resembles
        the curve near <m> x = a </m>.
          </p>
        </li>

        <li permid="OwI">
          <p permid="rJl">
        The equation for the tangent line of <m> f(x) </m> at <m> x = a </m> is 
        <me>y = f'(a)(x-a) + f(a), </me> 
        and so the necessary information to find is the value of the function at <m> x = a </m>, 
        the derivative <m> f'(x) </m>, and the value of the derivative at <m> x=a </m>.
          </p>
        </li>
      </ul>
    </p>
  </subsection>

<exercises xmlns:xi="http://www.w3.org/2001/XInclude"> 

  <exercise>
    <title>Sign of tangent line slope</title>
    <webwork source="UNL-Problems/104-Problems/tan_line_graph_1.pg" />
  </exercise>

  <exercise>
    <title>Sign of tangent line slope</title>
    <webwork source="UNL-Problems/104-Problems/tan_line_graph_2.pg" />
  </exercise>
  
  <exercise>
    <title>Equation of tangent line for polynomial</title>
    <webwork source="UNL-Problems/104-Problems/derivative_rules10.pg" />
  </exercise>

  <exercise>
    <title>Equation of tangent line for polynomial</title>
    <webwork source="UNL-Problems/104-Problems/derivative_rules8.pg" />
  </exercise>

  <exercise>
    <title>Equation of tangent line for non-polynomial</title>
    <webwork source="UNL-Problems/104-Problems/derivative_rules9.pg" />
  </exercise>

  <exercise>
    <title>Equation of tangent line for non-polynomial</title>
    <webwork source="UNL-Problems/104-Problems/tan_line_1.pg" />
  </exercise>

  <exercise>
    <title>Equation of tangent line</title>
    <webwork source="UNL-Problems/104-Problems/tan_line_2.pg" />
  </exercise>

 </exercises>
</section>

